start hw3.v over...

homework03/hw3/.CoqMakefile.d
@@ -1,0 +1,4 @@
+hw3.vo hw3.glob hw3.v.beautified hw3.required_vo: hw3.v imp.vo
+hw3.vos hw3.vok hw3.required_vos: hw3.v imp.vos
+imp.vo imp.glob imp.v.beautified imp.required_vo: imp.v 
+imp.vos imp.vok imp.required_vos: imp.v 
